TestModels/resources/src/Index.dfy
@@ -1,0 +1,68 @@
+// Copyright Amazon.com Inc. or its affiliates. All Rights Reserved.
+// SPDX-License-Identifier: Apache-2.0
+
+include "../Model/SimpleResourcesTypes.dfy"
+include "./Config.dfy"
+include "./SimpleResourcesOperations.dfy"
+
+module SimpleResources refines AbstractSimpleResourcesService
+{
+  import Operations = SimpleResourcesOperations
+  import Config
+
+  function method DefaultSimpleResourcesConfig(): SimpleResourcesConfig
+  {
+    SimpleResourcesConfig(
+      name := "default"
+    )
+  }
+
+  method SimpleResources(
+    config: SimpleResourcesConfig
+  ) returns (
+    res: Result<SimpleResourcesClient, Error>
+  )
+    ensures
+      res.Success?
+    ==>
+      && |config.name| > 0
+      && fresh(res.value.Modifies)
+      && fresh(res.value.History)
+      && res.value.ValidState()
+      && Operations.ValidInternalConfig?(res.value.config)
+  {
+    :- Need(|config.name| > 0,
+      Types.SimpleResourceException(
+      message := "Length of name must be greater than 0")
+    );
+    var internalConfig: Operations.InternalConfig := Config.Config(
+      name := config.name
+    );
+
+    var client := new SimpleResourcesClient(
+      config := internalConfig
+    );
+
+    return Success(client);  
+  }
+
+  class SimpleResourcesClient...
+  {
+    predicate ValidState()
+    {
+      && Operations.ValidInternalConfig?(config)
+      && History !in Operations.ModifiesInternalConfig(config)
+      && Modifies == Operations.ModifiesInternalConfig(config) + {History}
+    }
+
+    constructor(
+      config: Operations.InternalConfig
+    )
+    {
+      this.config := config;
+      History := new ISimpleResourcesClientCallHistory();
+      Modifies := Operations.ModifiesInternalConfig(config) + {History};
+    }
+  }
+}
+  
